\begin{frame}
\frametitle{Properties of $\bf{\alpha}$~and $\bf{\beta}$ }
\[
\alpha_x^2 p_x^2 + \alpha_y^2 p_y^2 + \alpha_z^2 p_z^2 + \beta^2 m^2 = p_x^2 + p_y^2 + p_z^2 + m^2
\]
Implies

%\begin{empheq}[box=\tcbhighmath]{align}
%a&=b\\
%E&=mc^2 + \int_a^a x\, dx
%\end{empheq}

\begin{empheq}[box=\tcbhighmath]{align}
\alpha_x^2 = \alpha_y^2 = \alpha_z^2 = \beta^2 = 1
\end{empheq}

%\end{block}

Define the anticommutator symbol as:
\[
\{A, B\} = AB + BA
\]

Then
\begin{align*}
& (\alpha_x \alpha_y + \alpha_y \alpha_x) p_x p_y 
+ (\alpha_x \alpha_z + \alpha_z \alpha_x) p_x p_z \\
+ & (\alpha_y \alpha_z + \alpha_y \alpha_y) p_y p_z 
+ (\alpha_x \beta + \beta \alpha_x) m p_x \\
+ & (\alpha_y \beta + \beta \alpha_y) m p_y 
+  (\alpha_z \beta + \beta \alpha_z) m p_z 
= 0
\end{align*}
Implies

\begin{empheq}[box=\tcbhighmath]{align}
\{\alpha_i, \alpha_j\}&=0 \, \, ( i \neq j)\\
\{\alpha_i, \beta\} & = 0
\end{empheq}

%\begin{align*}
%\{\alpha_i, \alpha_j\} = & 0 \, \, ( i \neq j) \\
%\{\alpha_i, \beta\} = & 0 
%
%\end{align*}

\end{frame}
